book/tutorial/Spec.Test.fst
@@ -1,0 +1,11 @@
+module Spec.Test
+
+/// It's really important to put spec tests in a separate module. Putting them
+/// in ``Spec.Bignum`` would mean their encoding in the SMT solver would be fed
+/// every time to Z3, polluting the context and slowing proofs down. Don't do that!
+
+module S = FStar.Seq
+module Spec = Spec.Bignum
+
+let test (): bool =
+  true
