book/Setup.rst
@@ -1,0 +1,165 @@
+Getting started
+===============
+
+For the sake of this tutorial, we use a sample project that provides a toy
+implementation of bignum addition in C. The project is located in the kremlin
+repository, under the ``book/tutorial`` directory.
+
+Installing the tools
+--------------------
+
+We recommend using the `Everest script
+<https://github.com/project-everest/everest>`_, if only for its ``z3`` and
+``opam`` commands, to make sure you have the exact version of the tools we need.
+All of our proofs are intimately tied to a specific version of F*, and if you're
+not running the right one, you may have trouble even building F*'s standard
+library.
+
+.. code-block:: bash
+
+  $ ./everest z3 opam
+
+Then, you can either install F* and KreMLin yourself, or rely on the Everest
+script for that purpose:
+
+.. code-block:: bash
+
+  $ ./everest pull FStar make kremlin make
+
+In any case, remember to export suitable values for the FSTAR_HOME and
+KREMLIN_HOME environment variables once you're done.
+
+Be aware that KreMLin is not at this time compatible with recent versions of
+OCaml. See `https://github.com/FStarLang/kremlin/issues/169`_ for the discussion.
+
+We strongly recommend using the fstar-mode.el Emacs plugin for interactive mode
+support. There is an extra customization step which allows querying a Makefile
+to figure out the arguments to pass to F*; please follow instructions at
+`https://github.com/project-everest/mitls-fstar#configuring-emacs-mode`_ -- this
+is used pretty pervasively throughout all of the Everest projects.
+
+Directory structure
+-------------------
+
+We adopt the following canonical and recommended structure for the toy project.
+
+- ``code``: low-level implementation in Low*, extracts to C
+- ``code/c``: hand-written C code (unverified), linked with the extracted Low*
+  code
+- ``specs``: high-level specifications, extract to OCaml for specs testing
+- ``specs/ml``: hand-written OCaml code (unverified), linked with the extracted
+  OCaml specifications
+- ``obj``: F* and OCaml build artifacts, i.e. whatever is covered by F*'s
+  ``--depend`` facility: ``.checked`` files (binary serialized build products
+  once a file has been verified), ``.ml`` files (the result of F* extracting to
+  OCaml), ``.krml`` files (the result of F* dumping its AST for KreMLin),
+  ``.cm*`` files (OCaml build), etc.
+- ``hints``: F* hint files, i.e. serialized Z3 unsat-cores that facilitate proof
+  replay
+- ``dist``: a distribution, i.e. a self-contained set of C files for clients to
+  check into their project.
+- ``tests``: hand-written C tests to make sure the generated code has a suitable
+  API.
+
+This toy project will thus illustrate mixing hand-written and generated ML and C
+files, a situation that is fairly common when working in Low*.
+
+Build
+-----
+
+Build is essential! This will be the entry point for any contributor to your
+project. A poorly designed build system will generate frustration, angst and
+conflict in the projet, while a well-ironed and smoothed-out build system will
+ensure bliss and happiness. Do not neglect your build system! It would be a
+mistake to think you can just copy-paste the reference Makefile provided below
+and then forget about it.
+
+Overview of a build
+^^^^^^^^^^^^^^^^^^^
+
+A quick word before showing our reference Makefile for the toy project.
+
+We advocate the usage of Makefiles (GNU), mostly because F* supports directly
+generating a .depend that will contain all the build rules for you. This is a
+well-debugged build system; other attempts at building F* projects with
+alternative build systems have failed.
+
+The build system of a Low* project operates in several phases:
+
+- dependency analysis of all F* source files, generating a ``.depend``
+- verify all the source files for this project, generating ``.checked`` files
+- extract F* code using those checked files to either ``.krml`` or ``.ml``
+- build and link ML code (for specs)
+- run KreMLin and generate C code
+- dependency analysis for the generated C code
+- build C code, generating a C library (more rarely, an executable)
+- build C tests and link against compiled library.
+
+To limit the amount of complexity, we only recursively execute ``make`` when a
+new dependency analysis needs to be performed. This means that C code
+compilation will be a sub-make, but everything is tied together in a single
+Makefile. In short, our Makefile has only two stages.
+
+.. note::
+
+  As a point of comparison, the HACL* Makefile has more stages: an initial one
+  that runs the Vale tool to generate F* files, a second stage (F* compilation &
+  extraction to C), a third stage (compilation of generated C code and ctypes
+  bindings generation code), a fourth stage (execution then compilation of the
+  generated Ctypes OCaml bindings), and perhaps a few more.
+
+In particular, F* will generate dependency information in ``.depend`` for the
+generation of ``.krml`` and ``.ml`` files, but will also generate a build graph
+for the resulting ``.cm*`` files, i.e. there is no need to run ``ocamldep``, as
+F* generates the information for you. This saves a recursive build.
+
+.. note::
+
+  you could conceivably extract all the ``.ml`` files to a separate directory
+  and use an external build tool, e.g. ``dune`` -- this is not covered here
+
+Modularity across projects
+^^^^^^^^^^^^^^^^^^^^^^^^^^
+
+Each project is expected to build its own .checked files; running ``make`` in
+``FStar/`` establishes the invariant that all the checked files are up-to-date
+w.r.t. their respective source files; similarly, running make in ``kremlin/``
+ensures that all the ``kremlib`` (C support libraries) .checked files are
+up-to-date.
+
+Any Low* program will need to refer to both ulib in F* and kremlib in KreMLin.
+The client Makefile we provide will therefore *enforce* that all the checked
+files for the projects it depends on be up-to-date, and will error out
+otherwise.
+
+The rationale is that the client project should not need to know how to build F*
+.checked files: there may be magic command-line flags, particular options, and
+special rules involved in the production of those checked files. If, say,
+``ulib/.cache/LowStar.Comment.fst.checked`` is out-of-date, then the user needs
+to rebuild F*.
+
+The same approach applies to the generated C code: each project should produce a
+library (by default, static, i.e. a ``.a`` file), and clients should link
+against that library. There are subtle problems related to C compilation,
+monomorphization and specialized types which are discussed later, but the short
+version is that a client never includes headers from the libraries it depends
+on; instead, kremlin re-generates signatures and projects are glued together at
+link-time.
+
+For instance, building kremlib generates ``kremlib/dist/generic/libkremlib.a``
+(more on multiple flavors of kremlib later). Our toy program will produce
+``libbignum.a``, without any reference to ``libkremlib.a``. C clients will link
+against both.
+
+.. todo::
+
+  kremlib somehow bypasses this approach by generating static headers with inline
+  static definitions, rather than generating externally-linked functions that are
+  reconciled at link-time (the previous approach). need to explain this
+
+Reference Makefile
+^^^^^^^^^^^^^^^^^^
+
+.. literalinclude:: tutorial/Makefile
+    :language: make
+
